theories/examples/loadstore.v
@@ -1,5 +1,7 @@
 From Forq Require Import Auto.
 From Forq.Words Require Import Core.
+From Forq.ProofRules Require Import Hoare.
+From Forq.ProofRules.Words Require Import Core.
 
 Module ST := State CoreSyntax.
 Module SMX := CoreSemantics ST.
@@ -26,7 +28,10 @@ Proof.
     constructor.
     now cbv [mem].
   simpl. eapply PMStepMulti.
-    constructor. reflexivity.
+    constructor.
+    cbv [mem]. now apply mem_well_typed_update.
+  simpl. eapply PMStepMulti.
+    constructor.
     cbv [mem]. now apply mem_well_typed_update.
   simpl. eapply PMStepMulti.
     constructor.
@@ -35,10 +40,7 @@ Proof.
     constructor.
     cbv [mem]. now apply mem_well_typed_update.
   simpl. eapply PMStepMulti.
-    constructor. reflexivity.
-    cbv [mem]. now apply mem_well_typed_update.
-  simpl. eapply PMStepMulti.
-    constructor. reflexivity.
+    constructor.
     cbv [mem]. apply mem_well_typed_update.
       now apply mem_well_typed_update.
       now rewrite update_eq.
@@ -61,3 +63,32 @@ Proof.
   (* store *)
   step ().
 Qed.
+
+Module CoreHoare := CoreHoare ST MM8.
+Import CoreHoare.
+
+Definition mem_wt : Assertion := fun st => PS.MM.mem_well_typed st.(mem).
+
+Theorem loadstore_correct'' : forall (a val : N),
+  {{ mem_wt }} loadstore a val {{ @@a = val }}.
+Proof.
+  intros. unfold loadstore.
+  (* store *)
+  eapply hoare_cons. eapply hoare_consequence_pre with
+      (Q := fun st => mem_wt st /\ exists tl, st.(stack) = a :: tl).
+    apply hoare_literal. intros st H.
+    unfold assertion_push_stack, mem_wt. simpl. split. assumption. exists st.(stack).
+    reflexivity.
+  eapply hoare_cons. eapply hoare_consequence_pre with
+      (Q := fun st => mem_wt st /\ exists tl, st.(stack) = val :: a :: tl).
+    apply hoare_literal. intros st (WT & t & St).
+    unfold assertion_push_stack, mem_wt. simpl. split. assumption. exists t. now rewrite St.
+  eapply hoare_cons with (Q := fun st => mem_wt st /\ exists (m : memT), st.(mem) = m[a := val]).
+  eapply hoare_consequence_pre. apply hoare_store with (addr := a) (val := val).
+    intros st (WT & t & St). split; ltac1:(cycle 1).
+    split. unfold mem_wt. simpl. (mem_well_typed_update (mem st) a val).
+  apply hoare_consequence_pre with
+    (P' := fun st =>
+      st.(stack) = val :: a :: nil /\
+      mem_wt[@a := val] {|stack := nil; mem := st.(mem)[a := val]; dict := st.(dict)|}).
+    apply hoare_store. intros st H. split.
