theories/Tactics.v
@@ -1,0 +1,16 @@
+From Ltac2 Require Import Ltac2.
+
+Ltac2 rec inv_list (hs : ident list) :=
+  match hs with
+  | [] => ()
+  | h :: hs' =>
+      ltac1:(h |- let h' := fresh h in
+        rename h into h'; inversion h'; clear h'; subst) (Ltac1.of_ident h);
+      inv_list hs'
+  end.
+
+Ltac2 Notation "inv" "[" hs(list1(ident)) "]" :=
+  inv_list hs.
+Ltac2 Notation "inv" hs(ident) :=
+  inv_list [hs].
+
